theories/typing.v
@@ -13,6 +13,10 @@ Section Typing.
   (* assume a given set of class definitions *)
   Context `{PDC: ProgDefContext}.
 
+  Hypothesis Δsdt_wf: ∀ A vars σ, Forall wf_ty σ → Forall wf_constraint (Δsdt A vars σ).
+  Hypothesis Δsdt_subst_ty: ∀ A vars σ0 σ,
+    subst_constraints σ (Δsdt A vars σ0) = Δsdt A vars (subst_ty σ <$> σ0).
+
   (* Helping the inference with this notation that hides pdefs *)
   Local Notation "Δ ⊢ s <: t" := (@subtype _ Δ Plain s t) (at level 70, s at next level, no associativity).
   Local Notation "Δ ⊢ s <D: t" := (@subtype _ Δ Aware s t) (at level 70, s at next level, no associativity).
@@ -47,7 +51,7 @@ Section Typing.
     - apply OkClass with def => //.
       + move => i ty h; by apply hi with i.
       + move => i c h.
-        apply subtype_weaken with Δ; by eauto.
+        apply subtype_weaken with Δ => //; by eauto.
     - constructor; by eauto.
     - constructor; by eauto.
   Qed.
@@ -85,7 +89,7 @@ Section Typing.
         rewrite /wf_cdef_constraints_bounded Forall_lookup in hdef'.
         assert (h' := h).
         apply hdef' in h as [].
-        apply subtype_weaken with (subst_constraints σ Δ); last by set_solver.
+        apply subtype_weaken with (subst_constraints σ Δ) => //; last by set_solver.
         rewrite -!subst_ty_subst.
         * apply subtype_subst => //.
           by apply hconstr with i.
@@ -771,28 +775,28 @@ Section Typing.
       else True) cdef.(classmethods)
   .
 
-  Definition wf_cdef_extends_dyn_targs def pdef σp :=
+  Definition wf_cdef_extends_dyn_targs t def tp pdef σp :=
     let σ := gen_targs (length def.(generics)) in
-    ∀ k c, (Δsdt def.(generics) σ) !! k = Some c →
-    def.(constraints) ++ Δsdt pdef.(generics) σp ⊢ c.1 <D: c.2
+    Δentails Aware (def.(constraints) ++ Δsdt tp pdef.(generics) σp)
+             (Δsdt t def.(generics) σ)
     .
 
-  Definition wf_cdef_extends_dyn def :=
+  Definition wf_cdef_extends_dyn t def :=
     match def.(superclass) with
     | None => True
     | Some (parent, σ) =>
         ∃ pdef, pdefs !! parent = Some pdef ∧
-        wf_cdef_extends_dyn_targs def pdef σ
+        wf_cdef_extends_dyn_targs t def parent pdef σ
     end.
 
   Lemma extends_using_extends_dyn A B σ:
     map_Forall (λ _ : string, wf_cdef_parent pdefs) pdefs →
-    map_Forall (λ _, wf_cdef_extends_dyn) pdefs →
+    map_Forall wf_cdef_extends_dyn pdefs →
     extends_using A B σ →
     ∃ adef bdef,
       pdefs !! A = Some adef ∧
       pdefs !! B = Some bdef ∧
-      wf_cdef_extends_dyn_targs adef bdef σ.
+      wf_cdef_extends_dyn_targs A adef B bdef σ.
   Proof.
     move => ? hwf hext.
     assert (hext0 := hext).
@@ -809,18 +813,18 @@ Section Typing.
   Lemma inherits_using_extends_dyn A B σ:
     map_Forall (λ _ : string, wf_cdef_parent pdefs) pdefs →
     map_Forall (λ _cname, wf_cdef_parent_ok) pdefs →
-    map_Forall (λ _, wf_cdef_extends_dyn) pdefs →
+    map_Forall wf_cdef_extends_dyn pdefs →
     inherits_using A B σ →
     ∃ adef bdef,
       pdefs !! A = Some adef ∧
       pdefs !! B = Some bdef ∧
-      wf_cdef_extends_dyn_targs adef bdef σ.
+      wf_cdef_extends_dyn_targs A adef B bdef σ.
   Proof.
     move => ? hok hwf.
     induction 1 as [ A adef hpdefs | A B σ hext | A B σ C σC hext h hi ].
     - exists adef, adef; repeat split => //.
       move => k [??] heq.
-      eapply subtype_weaken.
+      eapply subtype_weaken; [done | done | | ].
       + apply SubConstraint.
         by apply elem_of_list_lookup_2 with k.
       + by set_solver.
@@ -847,42 +851,41 @@ Section Typing.
       destruct (adef.(constraints) !! k) as [[??] | ] eqn:hc0.
       { rewrite hc0 in heq.
         case : heq => <-.
-        eapply subtype_weaken.
+        eapply subtype_weaken; [ done | done | | ].
         - apply SubConstraint.
           apply elem_of_list_lookup_2 with k.
           by apply hc0.
         - by set_solver.
       }
       rewrite hc0 in heq.
-      pose (k' := k - length adef.(generics)).
-      replace (Δsdt bdef.(generics) σ) with
-              (subst_constraints σ (Δsdt bdef.(generics) (gen_targs (length bdef.(generics)))))
+      replace (Δsdt B bdef.(generics) σ) with
+              (subst_constraints σ (Δsdt B bdef.(generics) (gen_targs (length bdef.(generics)))))
               in heq;last first.
       { by rewrite Δsdt_subst_ty subst_ty_gen_targs. }
       apply list_lookup_fmap_inv in heq as [c1 [-> hc1]].
       simpl.
       apply subtype_constraint_trans with
-        ((subst_constraints σ bdef.(constraints)) ++ Δsdt cdef.(generics) (subst_ty σ <$> σC));
+        ((subst_constraints σ bdef.(constraints)) ++ Δsdt C cdef.(generics) (subst_ty σ <$> σC));
         last first.
       { move => i c hc.
         rewrite lookup_app in hc.
         destruct (subst_constraints σ bdef.(constraints) !! i) as [cc0 | ] eqn:hcc0.
         - case: hc => <-.
-          apply subtype_weaken with adef.(constraints); last by set_solver.
+          apply subtype_weaken with adef.(constraints); [done | done | | by set_solver].
           apply extends_using_ok in hext => //.
           apply list_lookup_fmap_inv in hcc0 as [? [-> hcc]].
           rewrite /subst_constraint /=.
           destruct hext as (? & ? & hhok); simplify_eq.
           inv hhok; simplify_eq.
           by eauto.
-        - eapply subtype_weaken.
+        - eapply subtype_weaken; [ done | done | | ].
           + apply SubConstraint.
             eapply elem_of_list_lookup_2.
             destruct c; by apply hc.
           + by set_solver.
       }
-      replace (subst_constraints σ bdef.(constraints) ++ Δsdt cdef.(generics) (subst_ty σ <$> σC)) with
-              (subst_constraints σ (bdef.(constraints) ++ Δsdt cdef.(generics) σC)); last first.
+      replace (subst_constraints σ bdef.(constraints) ++ Δsdt C cdef.(generics) (subst_ty σ <$> σC)) with
+              (subst_constraints σ (bdef.(constraints) ++ Δsdt C cdef.(generics) σC)); last first.
       { rewrite /subst_constraints fmap_app.
         f_equal.
         by rewrite -Δsdt_subst_ty.
@@ -901,7 +904,7 @@ Section Typing.
   Definition wf_cdef_fields_dyn_wf cname cdef :=
     let n := length cdef.(generics) in
     let σ := gen_targs n in
-    let Δ := cdef.(constraints) ++ Δsdt cdef.(generics) σ in
+    let Δ := cdef.(constraints) ++ Δsdt cname cdef.(generics) σ in
     if cdef.(support_dynamic) then
     ∀ fields, has_fields cname fields →
     map_Forall (λ _fname vfty, wf_field_dyn_wf Δ vfty) fields
@@ -965,7 +968,7 @@ Section Typing.
    *)
   Record wf_cdefs (prog: stringmap classDef) := {
     wf_extends_wf : wf_no_cycle prog;
-    wf_extends_dyn : map_Forall (λ _, wf_cdef_extends_dyn) prog;
+    wf_extends_dyn : map_Forall wf_cdef_extends_dyn prog;
     wf_parent : map_Forall (λ _cname, wf_cdef_parent prog) prog;
     wf_parent_ok : map_Forall (λ _cname, wf_cdef_parent_ok) prog;
     wf_constraints_wf : map_Forall (λ _cname, wf_cdef_constraints_wf) prog;
