theories/soundness/dyn_getc.v
@@ -20,6 +20,18 @@ Section proofs.
   (* Iris semantic context *)
   Context `{!sem_heapGS Θ}.
 
+  Hypothesis Δsdt_wf: ∀ A vars σ, Forall wf_ty σ → Forall wf_constraint (Δsdt A vars σ).
+  Hypothesis Δsdt_subst_ty: ∀ A vars σ0 σ,
+    subst_constraints σ (Δsdt A vars σ0) = Δsdt A vars (subst_ty σ <$> σ0).
+  Hypothesis Δsdt_bounded: ∀ A vars σ n,
+    Forall (bounded n) σ →
+    Forall (bounded_constraint n) (Δsdt A vars σ).
+  Hypothesis Δsdt_lift: ∀ n A vars σ,
+    lift_constraints n (Δsdt A vars σ) = Δsdt A vars (lift_ty n <$> σ).
+  Hypothesis Δsdt_variance: ∀ Δ kd A vars σ0 σ1,
+    subtype_targs Δ kd vars σ0 σ1 →
+    Δentails kd (Δ ++ Δsdt A vars σ1) (Δsdt A vars σ0).
+
   (* Helping the inference with this notation that hides pdefs *)
   Local Notation "Δ ⊢ s <: t" := (@subtype _ Δ Plain s t) (at level 70, s at next level, no associativity).
   Local Notation "Δ ⊢ s <D: t" := (@subtype _ Δ Aware s t) (at level 70, s at next level, no associativity).
@@ -71,10 +83,10 @@ Section proofs.
       destruct hinherits as (?&?&?&hh).
       inv hh; by simplify_eq.
     }
-    pose (Δdyn0 := Δsdt def0.(generics) (gen_targs (length def0.(generics)))).
-    pose (Δdyn := Δsdt dyndef.(generics) σ).
-    assert (hnewcond: ∀ k c, Δdyn0 !! k = Some c → def0.(constraints) ++ Δdyn ⊢ c.1 <D: c.2).
-    { apply inherits_using_extends_dyn in hinherits; try by apply wfpdefs.
+    pose (Δdyn0 := Δsdt t0 def0.(generics) (gen_targs (length def0.(generics)))).
+    pose (Δdyn := Δsdt dyntag dyndef.(generics) σ).
+    assert (hnewcond: Δentails Aware (def0.(constraints) ++ Δdyn) Δdyn0).
+    { apply inherits_using_extends_dyn in hinherits => //; try by apply wfpdefs.
       destruct hinherits as (def0' & ? & hdef0' & ? & hwf); simplify_eq.
       move => k c hc.
       by apply hwf with k.
@@ -112,7 +124,7 @@ Section proofs.
         rewrite lookup_app in hc.
         destruct (constraints def0 !! i) as [[??] | ] eqn:h0.
         - rewrite h0 in hc; case: hc => <-.
-          eapply subtype_weaken.
+          eapply subtype_weaken; [ done | done | | ].
           + apply SubConstraint.
             apply elem_of_list_lookup_2 with i.
             by apply h0.
@@ -129,122 +141,40 @@ Section proofs.
         by apply wf_ty_class_inv in hwf.
       }
       assert (hwf_ : Forall wf_constraint (def0.(constraints) ++ Δdyn)).
-      { apply Forall_app; by split.
-      }
+      { apply Forall_app; by split.  }
       iNext.
+      assert (hwfσ : Forall wf_ty σ).
+      { apply inherits_using_wf in hinherits => //.
+        destruct hinherits as (? & ? & ? & hh).
+        by apply wf_ty_class_inv in hh.
+      }
+      iAssert (interp_env_as_mixed Σdyn) as "hmixed1"; first by admit.
+      iAssert (interp_env_as_mixed (interp_list Σt σ)) as "hmixed0".
+      { iIntros (k phi hk w) "hphi".
+        apply list_lookup_fmap_inv in hk as [ty0 [-> hty0]].
+        rewrite -(interp_type_unfold Σt MixedT w).
+        iApply (submixed_is_inclusion_aux Σt ty0 w) => //.
+        rewrite Forall_lookup in hwfσ.
+        by apply hwfσ in hty0.
+      }
       iAssert (□ Σinterp Σt Δdyn)%I as "#hconstr_dyn".
-      { iClear "Hle hmixed hconstr hdyn H◯ Hh HΦ H H▷".
-        iModIntro; iIntros (i c hc w) "#h".
-        apply Δsdt_lookup_Some in hc as (k & var & ty & hvk & htk & hk).
-        iDestruct ("HΣdyn" $! k var hvk) as (ϕ) "[hϕ hiϕ]"; iClear "HΣdyn".
-        case : var hvk hk => hvk.
-        - case => [-> | ->] /=.
-          * iDestruct ("hiϕ" $! w) as "[h0 _]"; iClear "hiϕ".
-            rewrite !interp_dynamic_unfold; iApply "h0"; iClear "h0".
-            replace ty with (subst_ty σ (GenT k)); last by rewrite /= htk.
-            rewrite interp_type_subst; last first.
-            { apply lookup_lt_Some in htk.
-              by constructor.
-            }
-            iAssert (Σdyn !! k ≡ Some (interp_type (GenT k) Σdyn))%I as "hϕi".
-            { destruct (Σdyn !! k) as [? | ] eqn:heq.
-              - rewrite !option_equivI.
-                iPureIntro => w'.
-                by rewrite interp_generic_unfold /interp_generic heq /=.
-              - apply lookup_ge_None_1 in heq.
-                apply lookup_lt_Some in htk.
-                rewrite hlen hl0 in heq.
-                apply lt_not_le in htk.
-                by apply htk in heq.
-            }
-            iRewrite "hϕ" in "hϕi".
-            rewrite !option_equivI.
-            iRewrite "hϕi".
-            assert (hmono : mono dyndef.(generics) (GenT k)).
-            { by constructor. }
-            by iApply interp_with_mono.
-          * iDestruct ("hiϕ" $! w) as "[_ h0]"; iClear "hiϕ".
-            replace ty with (subst_ty σ (GenT k)); last by rewrite /= htk.
-            rewrite interp_type_subst; last first.
-            { apply lookup_lt_Some in htk.
-              by constructor.
-            }
-            rewrite !interp_dynamic_unfold.
-            iDestruct ("h0" with "h") as "h1"; iClear "h0 h".
-            iAssert (Σdyn !! k ≡ Some (interp_type (GenT k) Σdyn))%I as "hϕi".
-            { destruct (Σdyn !! k) as [? | ] eqn:heq.
-              - rewrite !option_equivI.
-                iPureIntro => w'.
-                by rewrite interp_generic_unfold /interp_generic heq /=.
-              - apply lookup_ge_None_1 in heq.
-                apply lookup_lt_Some in htk.
-                rewrite hlen hl0 in heq.
-                apply lt_not_le in htk.
-                by apply htk in heq.
-            }
-            iRewrite "hϕ" in "hϕi".
-            rewrite !option_equivI.
-            iRewrite "hϕi" in "h1"; iClear "hϕi".
-            iDestruct (neg_interp_variance with "hf0") as "hf1"; iClear "hf0".
-            assert (hmono : mono (neg_variance <$> dyndef.(generics)) (GenT k)).
-            { constructor.
-              by rewrite list_lookup_fmap hvk.
-            }
-            by iApply interp_with_mono.
-        - move => ->.
-          iSpecialize ("hiϕ" $! w).
-          rewrite /= !interp_dynamic_unfold; iApply "hiϕ".
-          replace ty with (subst_ty σ (GenT k)); last by rewrite /= htk.
-          rewrite interp_type_subst; last first.
-          { apply lookup_lt_Some in htk.
-            by constructor.
-          }
-          iAssert (Σdyn !! k ≡ Some (interp_type (GenT k) Σdyn))%I as "hϕi".
-          { destruct (Σdyn !! k) as [? | ] eqn:heq.
-            - rewrite !option_equivI.
-              iPureIntro => w'.
-              by rewrite interp_generic_unfold /interp_generic heq /=.
-            - apply lookup_ge_None_1 in heq.
-              apply lookup_lt_Some in htk.
-              rewrite hlen hl0 in heq.
-              apply lt_not_le in htk.
-              by apply htk in heq.
-          }
-          iRewrite "hϕ" in "hϕi".
-          rewrite !option_equivI.
-          iRewrite "hϕi".
-          assert (hmono : mono dyndef.(generics) (GenT k)).
-          { by constructor. }
-          by iApply interp_with_mono.
-        - move => ->.
-          iSpecialize ("hiϕ" $! w).
-          replace ty with (subst_ty σ (GenT k)); last by rewrite /= htk.
-          rewrite interp_type_subst; last first.
-          { apply lookup_lt_Some in htk.
-            by constructor.
-          }
-          rewrite !interp_dynamic_unfold.
-          iDestruct ("hiϕ" with "h") as "h1".
-          iAssert (Σdyn !! k ≡ Some (interp_type (GenT k) Σdyn))%I as "hϕi".
-          { destruct (Σdyn !! k) as [? | ] eqn:heq.
-            - rewrite !option_equivI.
-              iPureIntro => w'.
-              by rewrite interp_generic_unfold /interp_generic heq /=.
-            - apply lookup_ge_None_1 in heq.
-              apply lookup_lt_Some in htk.
-              rewrite hlen hl0 in heq.
-              apply lt_not_le in htk.
-              by apply htk in heq.
-          }
-          iRewrite "hϕ" in "hϕi".
-          rewrite !option_equivI.
-          iRewrite "hϕi" in "h1"; iClear "hϕi".
-          iDestruct (neg_interp_variance with "hf0") as "hf1"; iClear "hf0".
-          assert (hmono : mono (neg_variance <$> dyndef.(generics)) (GenT k)).
-          { apply MonoVCoGen.
-            by rewrite list_lookup_fmap hvk.
-          }
-          by iApply interp_with_mono.
+      { iClear "Hle hconstr hdyn H◯ Hh HΦ H H▷".
+        iModIntro; iIntros (i c0 hc w) "#h".
+        rewrite /Δdyn -(subst_ty_gen_targs (length dyndef.(generics)) σ) // in hc.
+        rewrite -Δsdt_subst_ty in hc.
+        apply list_lookup_fmap_inv in hc as [c [-> hc]] => /=.
+        assert (hbc : bounded_constraint (length σ) c).
+        { rewrite -hl0.
+          move : (bounded_gen_targs (length dyndef.(generics))) => hh.
+          apply Δsdt_bounded with (A := dyntag) (vars := dyndef.(generics)) in hh.
+          rewrite Forall_lookup in hh.
+          by apply hh in hc.
+        }
+        destruct hbc as [].
+        rewrite !interp_type_subst //.
+        by iApply ((Δsdt_variance_interp Δsdt_wf Δsdt_subst_ty Δsdt_bounded
+          Δsdt_lift Δsdt_variance _ _ _ _ wf_mono wf_parent hdyndef)
+          with "hmixed0 hmixed1 hf0 HΣdyn").
       }
       iAssert (□ Σinterp Σt (constraints def0 ++ Δdyn))%I as "hconstr_".
       { iModIntro.
@@ -256,7 +186,7 @@ Section proofs.
       iSpecialize ("h" $! name _ with "[hdyn]"); first done.
       iDestruct "h" as (w) "[%hw hiw]".
       simplify_eq.
-      iDestruct (subtype_is_inclusion _ hwf_ wf_parent wf_mono _ Σt _ _ hsub' v) as "hsub".
+      iDestruct (subtype_is_inclusion _ _ _ _ hwf_ wf_parent wf_mono _ Σt _ _ hsub' v) as "hsub".
       { by apply has_field_wf in hf. }
       by iApply "hsub".
     }
