theories/subtype.v
@@ -13,133 +13,12 @@ Section Subtype.
   (* assume a given set of class definitions *)
   Context `{PDC: ProgDefContext}.
 
+  Parameter Δsdt : tag → list variance → list lang_ty → list constraint.
+  Hypothesis Δsdt_wf: ∀ A vars σ, Forall wf_ty σ → Forall wf_constraint (Δsdt A vars σ).
+  Hypothesis Δsdt_subst_ty: ∀ A vars σ0 σ,
+    subst_constraints σ (Δsdt A vars σ0) = Δsdt A vars (subst_ty σ <$> σ0).
+
   Inductive subtype_kind := Aware | Plain.
-
-  Definition Δsdt (vars: list variance) σ : list constraint :=
-    let l := zip_with
-      (λ var ty, match var with
-                  | Covariant => [(ty, DynamicT)]
-                  | Contravariant => [(DynamicT, ty)]
-                  | Invariant => [(ty, DynamicT); (DynamicT, ty)]
-                  end) vars σ in
-    concat l.
-
-  Lemma Δsdt_wf vars σ : Forall wf_ty σ → Forall wf_constraint (Δsdt vars σ).
-  Proof.
-    move/Forall_lookup => h.
-    apply Forall_concat.
-    apply Forall_lookup => i ?.
-    rewrite lookup_zip_with_Some => [[var] [ty [-> [hvar hty]]]].
-    apply h in hty.
-    by destruct var; by repeat constructor.
-  Qed.
-
-  (* Lemma Δsdt_wf σ : Forall wf_ty σ → Forall wf_constraint (Δsdt σ). *)
-  (* Proof. *)
-  (*   move/Forall_lookup => h. *)
-  (*   apply Forall_lookup => i ? heq. *)
-  (*   apply list_lookup_fmap_inv in heq as [c [-> hc]]. *)
-  (*   split; last done. *)
-  (*   by apply h in hc. *)
-  (* Qed. *)
-
-  Lemma Δsdt_subst_ty vars: ∀ (σ0 σ: list lang_ty),
-    subst_constraints σ (Δsdt vars σ0) = Δsdt vars (subst_ty σ <$> σ0).
-  Proof.
-    elim : vars => [ | hd tl hi] σ0 σ //=.
-    case : σ0 => [ | ty0 σ0] //=.
-    rewrite /subst_constraints /Δsdt /=.
-    case : hd => /=.
-    - f_equal.
-      f_equal.
-      by apply hi.
-    - f_equal.
-      f_equal.
-      by apply hi.
-    - f_equal.
-      f_equal.
-      by apply hi.
-  Qed.
-
-  (* Lemma Δsdt_subst_ty (σ0 σ: list lang_ty): *)
-  (*   subst_constraints σ (Δsdt σ0) = Δsdt (subst_ty σ <$> σ0). *)
-  (* Proof. *)
-  (*   apply list_eq => k. *)
-  (*   rewrite /subst_constraints /Δsdt !list_lookup_fmap. *)
-  (*   by destruct (σ0 !! k). *)
-  (* Qed. *)
-
-  Lemma Δsdt_lookup vars:
-    ∀ var σ k ty, vars !! k = Some var → σ !! k = Some ty →
-    match var with
-    | Invariant =>
-        ∃ i, (Δsdt vars σ) !! i = Some (ty, DynamicT) ∧
-             (Δsdt vars σ) !! (S i) = Some (DynamicT, ty)
-    | Covariant => 
-        ∃ i, (Δsdt vars σ) !! i = Some (ty, DynamicT)
-    | Contravariant => 
-        ∃ i, (Δsdt vars σ) !! i = Some (DynamicT, ty)
-    end.
-  Proof.
-    elim: vars => [ | hd tl hi] var σ k ty h0 h1 //=.
-    case : σ h1 => [ | ty0 σ] h1 //=.
-    case : k h0 h1 => [ | k] /= h0 h1.
-    - case : h0 => <-.
-      case : h1 => <-.
-      case : hd; by exists 0.
-    - move : {hi} (hi var σ k ty h0 h1) => h.
-      case: var h0 h1 h => h0 h1. 
-      + case => i [hi0 hi1].
-        case: hd.
-        * by exists (S (S i)).
-        * by exists (S i).
-        * by exists (S i).
-      + case => i hi.
-        case: hd.
-        * by exists (S (S i)).
-        * by exists (S i).
-        * by exists (S i).
-      + case => i hi.
-        case: hd.
-        * by exists (S (S i)).
-        * by exists (S i).
-        * by exists (S i).
-  Qed.
-
-  Lemma Δsdt_lookup_Some vars: ∀ σ k c,
-    (Δsdt vars σ) !! k = Some c →
-    ∃ i var ty, vars !! i = Some var ∧ σ !! i = Some ty ∧
-    match var with
-    | Invariant => c = (ty, DynamicT) ∨ c = (DynamicT, ty)
-    | Covariant => c = (ty, DynamicT)
-    | Contravariant => c = (DynamicT, ty)
-    end.
-  Proof.
-    elim : vars => [ | hd tl hi] σ k c heq //=.
-    case : σ heq => [ | ty σ] heq //=.
-    case : k heq => [ | k] //=.
-    - rewrite /Δsdt /= => heq.
-      exists 0, hd, ty; repeat split => //.
-      case : hd heq => /=.
-      + case => <-; by left.
-      + by case => <-.
-      + by case => <-.
-    - rewrite /Δsdt /= => heq.
-      case : hd heq => /=.
-      + case : k => [ | k] /=.
-        * case => <-.
-          exists 0, Invariant, ty.
-          by firstorder.
-        * move => h.
-          apply hi in h as (i & var & ty' & hv & ht & h).
-          by exists (S i), var, ty'.
-      + move => h.
-        apply hi in h as (i & var & ty' & hv & ht & h).
-        by exists (S i), var, ty'.
-      + move => h.
-        apply hi in h as (i & var & ty' & hv & ht & h).
-        by exists (S i), var, ty'.
-  Qed.
 
   (* Type well-formdness is mostly introduced to be able to define
    * subtyping rule correctly, like unions.
@@ -174,7 +53,7 @@ Section Subtype.
     | SubClassDyn: ∀ kd A adef σA,
         pdefs !! A = Some adef →
         adef.(support_dynamic) = true →
-        (∀ k s t, (Δsdt adef.(generics) σA) !! k = Some (s, t) → subtype Δ kd s t) →
+        (∀ k s t, (Δsdt A adef.(generics) σA) !! k = Some (s, t) → subtype Δ kd s t) →
         subtype Δ kd (ClassT A σA) SupportDynT
     | SubIntDyn kd: subtype Δ kd IntT SupportDynT
     | SubBoolDyn kd: subtype Δ kd BoolT SupportDynT
@@ -842,64 +721,8 @@ Section Subtype.
       by repeat split => //.
   Qed.
 
-  (*
-     Cov:
-     T_0 <: T_1 /\ Delta_C[T_0/T] /\ Delta_C[T_1/C] /\ Delta^SDT_C[T_1/T]
-     => Delta^SDT_C[T_0/T]
-     contra 
-  T_0 <: T_1 /\ Delta_C[T_0/T] /\ Delta_C[T_1/C] /\ Delta^SDT_C[T_0/T]
-    => Delta^SDT_C[T_1/T]
-   *)
   Definition Δentails kd (Δ0 Δ1: list constraint) :=
     ∀ i c, Δ1 !! i = Some c → subtype Δ0 kd c.1 c.2.
-
-  Lemma Δsdt_variance Δ kd vars σ0 σ1:
-    subtype_targs Δ kd vars σ0 σ1 →
-    Δentails kd (Δ ++ Δsdt vars σ1) (Δsdt vars σ0).
-  Proof.
-    induction 1 as [ kd | kd ty0 ty1 vs ty0s ty1s h0 h1 h hi | kd ty0 ty1 vs ty0s ty1s h0 h hi
-    | kd ty0 ty1 vs ty0s ty1s h0 h hi] => i c //=.
-    - case : i => [ | [ | i]] /= heq.
-      + case : heq => <- /=.
-        apply SubTrans with ty1.
-        * apply subtype_weaken with Δ => //.
-          by set_solver.
-        * apply SubConstraint.
-          apply elem_of_app; right.
-          by apply elem_of_list_lookup_2 with 0.
-      + case : heq => <- /=.
-        apply SubTrans with ty1.
-        * apply SubConstraint.
-          apply elem_of_app; right.
-          by apply elem_of_list_lookup_2 with 1.
-        * apply subtype_weaken with Δ => //.
-          by set_solver.
-      + apply hi in heq.
-        apply subtype_weaken with (Δ ++ Δsdt vs ty1s) => //.
-        by set_solver.
-    - case : i => [ | i] /= heq.
-      + case : heq => <- /=.
-        apply SubTrans with ty1.
-        * apply subtype_weaken with Δ => //.
-          by set_solver.
-        * apply SubConstraint.
-          apply elem_of_app; right.
-          by apply elem_of_list_lookup_2 with 0.
-      + apply hi in heq.
-        apply subtype_weaken with (Δ ++ Δsdt vs ty1s) => //.
-        by set_solver.
-    - case : i => [ | i] /= heq.
-      + case : heq => <- /=.
-        apply SubTrans with ty1.
-        * apply SubConstraint.
-          apply elem_of_app; right.
-          by apply elem_of_list_lookup_2 with 0.
-        * apply subtype_weaken with Δ => //.
-          by set_solver.
-      + apply hi in heq.
-        apply subtype_weaken with (Δ ++ Δsdt vs ty1s) => //.
-        by set_solver.
-  Qed.
 End Subtype.
 
 (* Hints and notations are local to the section. Re-exporting them *)
